Constaints.dfy
@@ -1,0 +1,3 @@
+module Constants {
+  const maxSize := 20;
+}
