cert_chain.dfy
@@ -1,0 +1,46 @@
+method set_certificate_chain(tls_opts : tls_opts, conn_ctx : tls_conn_ctx, filepath : string) returns (y : int)
+requires tls_opts != null;
+requires filepath != null;
+// ensures that there is a valid cetificate chain set afterward
+ensures y != 0;
+{
+  var cur_opts := new tls_opts;
+  if conn_ctx == null { // no connection yet
+    if tls_opts == null {
+      return 0; // y := 0
+    }
+    cur_opts = tls_opts;
+    if cur_opts->cur_opts == null {
+      // verify that filepath exists and has valid cert chain
+      // take filepath and load it into the SSL_CTX
+    }
+
+    else {
+        
+    }
+
+  }
+  else { // already has connection
+
+  }
+}
+
+class tls_conn_ctx
+{
+
+}
+
+class tls_opts 
+{
+//   SSL_CTX *tls_ctx
+// char *app_path
+// int custom_validation
+// int is_server
+// char alpn_string[ALPN_STRING_MAXLEN]
+// struct tls_opts* next
+}
+class SSL_CTX
+{
+// cert chain
+// x509 
+}
